Test/dafny0/NonGhostQuantifiers.dfy
@@ -1,0 +1,125 @@
+// This file contains various tests of resolving quantifiers in ghost and non-ghost positions
+
+class MyClass<T> {
+  // This function is in a ghost context, so all is cool.
+  function GhostF(): bool
+  {
+    (forall n :: 2 <= n ==> (exists d :: n < d && d < 2*n))
+  }
+  // But try to make it a non-ghost function, and Dafny will object because it cannot compile the
+  // body into code that will terminate.
+  function method NonGhostF(): bool
+  {
+    (forall n :: 2 <= n ==> (exists d :: n < d && d < 2*n))  // error: can't figure out how to compile
+  }
+  // Add an upper bound to n and things are cool again.
+  function method NonGhostF_Bounded(): bool
+  {
+    (forall n :: 2 <= n && n < 1000 ==> (exists d :: n < d && d < 2*n))
+  }
+  // Although the heuristics applied are syntactic, they do see through the structure of the boolean
+  // operators ==>, &&, ||, and !.  Hence, the following three variations of the previous function can
+  // also be compiled.
+  function method NonGhostF_Or(): bool
+  {
+    (forall n :: !(2 <= n && n < 1000) || (exists d :: n < d && d < 2*n))
+  }
+  function method NonGhostF_ImpliesImplies(): bool
+  {
+    (forall n :: 2 <= n ==> n < 1000 ==> (exists d :: n < d && d < 2*n))
+  }
+  function method NonGhostF_Shunting(): bool
+  {
+    (forall n :: 2 <= n ==> 1000 <= n || (exists d :: n < d && d < 2*n))
+  }
+
+  // Here are more tests
+
+  function method F(a: array<T>): bool
+    requires a != null;
+    reads a;
+  {
+    (exists i :: 0 <= i && i < a.Length / 2 && (forall j :: i <= j && j < a.Length ==> a[i] == a[j]))
+  }
+
+  function method G0(a: seq<T>): bool
+  {
+    (exists t :: t in a && (forall u :: u in a ==> u == t))
+  }
+  function method G1(a: seq<T>): bool
+  {
+    (exists ti :: 0 <= ti && ti < |a| && (forall ui :: 0 <= ui && ui < |a| ==> a[ui] == a[ti]))
+  }
+
+  // Regrettably, the heuristics don't know about transitivity:
+  function method IsSorted0(s: seq<int>): bool
+  {
+    (forall i, j :: 0 <= i && i < j && j < |s| ==> s[i] <= s[j])  // error: can't figure out how to compile
+  }
+  function method IsSorted1(s: seq<int>): bool
+  {
+    (forall j, i :: 0 <= i && i < j && j < |s| ==> s[i] <= s[j])  // error: can't figure out how to compile
+  }
+  // Add the redundant conjunct "i < |s|" and things are fine.
+  function method IsSorted2(s: seq<int>): bool
+  {
+    (forall i, j :: 0 <= i && i < |s| && i < j && j < |s| ==> s[i] <= s[j])
+  }
+  // But if you switch the order of i and j, you need a different redundant conjunct.
+  function method IsSorted3(s: seq<int>): bool
+  {
+    (forall j, i :: 0 <= i && i < |s| && i < j && j < |s| ==> s[i] <= s[j])  // error: can't figure out how to compile
+  }
+  function method IsSorted4(s: seq<int>): bool
+  {
+    (forall j, i  :: 0 <= i && 0 < j && i < j && j < |s| ==> s[i] <= s[j])
+  }
+
+  // The heuristics look at bound variables in the order given, as is illustrated by the following
+  // two functions.
+  function method Order0(S: seq<set<int>>): bool
+  {
+    (forall i, j :: 0 <= i && i < |S| && j in S[i] ==> 0 <= j)
+  }
+  function method Order1(S: seq<set<int>>): bool
+  {
+    (forall j, i :: 0 <= i && i < |S| && j in S[i] ==> 0 <= j)  // error: can't figure out how to compile
+  }
+
+  // Quantifiers can be used in other contexts, too.
+  // For example, in assert statements and assignment statements.
+  method M(s: seq<int>) returns (r: bool, q: bool) {
+    assert (forall x :: x in s ==> 0 <= x);
+    r := (forall x :: x in s ==> x < 100);
+    q := (exists y :: y*y in s);  // error: can't figure out how to compile
+  }
+  // And if expressions.
+  function method Select_Good(S: set<int>, a: T, b: T): T
+  {
+    if (forall x :: x in S ==> 0 <= x && x < 100) then a else b
+  }
+  function method Select_Bad(S: set<int>, a: T, b: T): T
+  {
+    if (forall x :: x*x in S ==> 0 <= x && x < 100) then a else b  // error: can't figure out how to compile
+  }
+  // (the same thing, but in a ghost function is fine, though)
+  function Select_Bad_Ghost(S: set<int>, a: T, b: T): T
+  {
+    if (forall x :: x*x in S ==> 0 <= x && x < 100) then a else b
+  }
+  // And if statements
+/****
+  method N(s: seq<int>) returns (ghost g: int, h: int)
+  {
+    if ( (forall x :: x in s ==> 0 <= x) ) {
+      h := 0;  g := 0;
+    }
+    if ( (forall x :: x*x in s ==> x < 100) ) {  // this is fine, since the whole statement is a ghost statement
+      g := 2;
+    }
+    if ( (forall x :: x*x in s ==> x < 50) ) {  // error: cannot compile this guard of a non-ghost if statement
+      h := 6;
+    }
+  }
+****/
+}
